Arbiter/Impl.v
@@ -1,213 +1,105 @@
-Require Import Kami.All.
+Require Import Kami.AllNotations.
 Require Import StdLibKami.Arbiter.Ifc.
-Require Import StdLibKami.FreeList.Ifc.
-Require Import List.
 
-Section ArbiterImpl.
-  Context {arbiterParams : ArbiterParams}.
+Section Impl.
+  Context {ifcParams : Ifc.Params}.
+  Context (clients : Clients).
 
-  Local Definition arbiterBusyRegName := (Arbiter.Ifc.name ++ ".busy")%string.
-  Local Definition arbiterAlistName   := (Arbiter.Ifc.name ++ ".alist")%string.
-  Local Definition arbiterAlistReadName  := (Arbiter.Ifc.name ++ ".alistRead")%string.
-  Local Definition arbiterAlistWriteName := (Arbiter.Ifc.name ++ ".alistWrite")%string.
+  Local Definition busyName := (name ++ ".busy")%string.
 
-  Instance freeListParams
-    :  FreeListParams 
-    := {|
-         name := (Arbiter.Ifc.name ++ ".freelist")%string;
-         tagSz := transactionTagSz;
-       |}.
+  Local Open Scope kami_expr.
+  Local Open Scope kami_action.
 
-  Class ArbiterImplParams :=
-    {
-      freelist: @FreeList freeListParams;
-    }.
-
-  Section withParams.
-    Context `{ArbiterImplParams}.
-
-    Local Open Scope kami_expr.
-    Local Open Scope kami_action.
-
-    Definition clientIdSz := Nat.log2_up numClients.
-    Definition ClientId := Bit clientIdSz.
-
-    Definition genericClientTagSz
-      := fold_left Nat.max
-           (map
-             (fun client : ArbiterClient _ _
-               => clientTagSz client)
-             clients)
-           0.
-
-    Definition genericClientTag := Bit genericClientTagSz.
-
-    Definition ClientIdTag
-      := STRUCT_TYPE {
-           "id"  :: ClientId;
-           "tag" :: genericClientTag
-         }.
-
-    Section withTy.
-      Definition nextToAlloc {ty: Kind -> Type} := @nextToAlloc _ freelist ty.
-      Definition alloc {ty: Kind -> Type} := @alloc _ freelist ty.
-      Definition free {ty: Kind -> Type}:= @free _ freelist ty.
-
-      (* Per-client translator request action *)
-
-      Open Scope kami_expr_scope.
-
-      Definition sendReq
-        (isError : forall {ty}, immResK @# ty -> Bool @# ty)
-        (routerSendReq
-          : forall {ty},
-            ty ArbiterRouterReq ->
-            ActionT ty (Maybe immResK))
-        (clientId : Fin.t numClients)
-        (ty : Kind -> Type)
-        (clientReq : ty (clientReqK (nth_Fin clients clientId)))
-        :  ActionT ty (Maybe immResK)
-        := System [
-             DispString _ "[Arbiter.sendReq] clientReq: ";
-             DispHex #clientReq;
-             DispString _ "\n"
-           ];
-           Read busy : Bool <- arbiterBusyRegName;
-           LETA transactionTag
-             :  Maybe TransactionTag
-             <- nextToAlloc;
+  Local Definition sendReq
+    (send: forall {ty}, ty (OutReq clients) -> ActionT ty (Maybe immResK))
+    (clientId : Fin.t (numClients clients))
+    (ty : Kind -> Type)
+    (clientReq : ty (ClientReq (clientTagSz (nth_Fin (clientList clients) clientId))))
+    :  ActionT ty (Maybe immResK)
+    := System [
+         DispString _ "[Arbiter.sendReq] clientReq: ";
+         DispHex #clientReq;
+         DispString _ "\n"
+       ];
+       Read busy : Bool <- busyName;
+       LET tag : (Tag clients) <- STRUCT {
+                                      "id"  ::= $(proj1_sig (Fin.to_nat clientId));
+                                      "tag" ::= ZeroExtendTruncLsb (maxClientTagSz clients) (#clientReq @% "tag")
+                                    };
+       System [
+         DispString _ "[Arbiter.sendReq] tag\n";
+         DispHex #tag;
+         DispString _ "\n"
+       ];
+       If !#busy
+         then
            System [
-             DispString _ "[Arbiter.sendReq] next available transaction tag\n";
-             DispHex #transactionTag;
-             DispString _ "\n"
+             DispString _ "[Arbiter.sendReq] sending request.\n"
            ];
-           If !#busy && #transactionTag @% "valid"
-             then
-               System [
-                 DispString _ "[Arbiter.sendReq] sending request.\n"
-               ];
-               Write arbiterBusyRegName : Bool <- $$true;
-               LET routerReq
-                 :  ArbiterRouterReq
-                 <- STRUCT {
-                      "tag" ::= #transactionTag @% "data";
-                      "req" ::= #clientReq @% "req"
-                    };
-               LETA routerImmRes
-                 :  Maybe immResK
-                 <- routerSendReq routerReq;
-               (* TODO: LLEE: accept an additional parameter that accepts an immres and returns true iff the immres signals an error. If error do not allocate resource (i.e. transaction tag. Note: this is a general error. Check other components as well. *) 
-               If #routerImmRes @% "valid" && !(isError (#routerImmRes @% "data"))
-                 then
-                   LET clientIdTag
-                     :  ClientIdTag
-                     <- STRUCT {
-                          "id"  ::= $(proj1_sig (Fin.to_nat clientId));
-                          "tag" ::= ZeroExtendTruncLsb genericClientTagSz (#clientReq @% "tag")
-                        };
-                   System [
-                     DispString _ "[Arbiter.sendReq] saving transaction and client req tag:\n";
-                     DispHex #clientIdTag;
-                     DispString _ "\n"
-                   ];
-                   WriteRf arbiterAlistWriteName (#transactionTag @% "data" : transactionTagSz ; #clientIdTag : ClientIdTag );
-                   LET transactionTagData
-                     :  TransactionTag
-                     <- #transactionTag @% "data";
-                   System [
-                     DispString _ "[Arbiter.sendReq] allocating transaction tag:\n";
-                     DispHex #transactionTagData;
-                     DispString _ "\n"
-                   ];
-                   alloc transactionTagData;
-               Ret #routerImmRes
-             else
-               Ret $$(getDefaultConst (Maybe immResK))
-             as result;
-           System [
-             DispString _ "[Arbiter.sendReq] result:";
-             DispHex #result;
-             DispString _ "\n"
-           ];
-           Ret #result.
+           Write busyName : Bool <- $$true;
+           LET outReq : (OutReq clients) <- STRUCT {
+                                                "tag" ::= #tag;
+                                                "req" ::= #clientReq @% "req"
+                                              };
+           LETA immResM : Maybe immResK <- send outReq;
+           Ret #immResM
+         else
+           Ret $$(getDefaultConst (Maybe immResK))
+         as ret;
+       System [
+         DispString _ "[Arbiter.sendReq] result:";
+         DispHex #ret;
+         DispString _ "\n"
+       ];
+       Ret #ret.
 
-      (*
-        What the "real" memory unit will call to respond to the tag
-        translator; This is where the routing of responses to individual
-        clients occurs.
-      *)
-      Definition memCallback
-        (ty: Kind -> Type)
-        (routerRes: ty ArbiterRouterRes)
-        :  ActionT ty Void
-        := System [
-             DispString _ "[Arbiter.memCallback] routerRes: ";
-             DispHex #routerRes;
-             DispString _ "\n"
-           ];
-           LET transactionTag
-             :  TransactionTag
-             <- #routerRes @% "tag";
-           ReadRf clientIdTag
-             :  ClientIdTag
-             <- arbiterAlistReadName (#transactionTag: TransactionTag);
-           LETA _
-             <- free transactionTag;
-           GatherActions
-             (map
-               (fun (clientId: Fin.t numClients)
-                 => let client
-                      :  ArbiterClient _ _
-                      := nth_Fin clients clientId in 
-                    If $(proj1_sig (Fin.to_nat clientId)) == (#clientIdTag @% "id")
-                      then
-                        LET clientRes
-                          :  clientResK client
-                          <- STRUCT {
-                               (* "tag"  ::= ZeroExtendTruncLsb (clientTagSz client) (#routerRes @% "tag"); (* TODO: LLEE: SOMETHINGS WRONG HERE *) *)
-                               "tag"  ::= ZeroExtendTruncLsb (clientTagSz client) (#clientIdTag @% "tag");
-                               "resp" ::= #routerRes @% "resp"
-                             };
-                        System [
-                          DispString _ "[Arbiter.memCallback] client res: ";
-                          DispHex #clientRes;
-                          DispString _ "\n"
-                        ];
-                        clientHandleRes client clientRes;
-                    Retv)
-               (getFins numClients))
-             as _;
-           Retv.
+  Local Definition callback
+    (ty: Kind -> Type)
+    (res: ty (InRes clients))
+    :  ActionT ty Void
+    := System [
+         DispString _ "[Arbiter.memCallback] res: ";
+         DispHex #res;
+         DispString _ "\n"
+       ];
+       LET clientIdTag <- #res @% "tag";
+       GatherActions
+         (map
+           (fun (clientId: Fin.t (numClients clients))
+             => let client: Client _ := nth_Fin (clientList clients) clientId in 
+                If $(proj1_sig (Fin.to_nat clientId)) == (#clientIdTag @% "id")
+                  then
+                    LET clientRes : clientResK client <- STRUCT {
+                                                             "tag"  ::= ZeroExtendTruncLsb (clientTagSz client)
+                                                                                           (#clientIdTag @% "tag");
+                                                             "res" ::= #res @% "res"
+                                                           };
+                    System [
+                      DispString _ "[Arbiter.memCallback] client res: ";
+                      DispHex #clientRes;
+                      DispString _ "\n"
+                    ];
+                    clientHandleRes client clientRes;
+                Retv)
+           (getFins (numClients clients)))
+         as _;
+       Retv.
 
-      (* TODO: LLEE does this make sense? *)
-      Definition arbiterRule ty : ActionT ty Void
-        := System [
-             DispString _ "[Arbiter.arbiterRule]\n"
-           ];
-           Write arbiterBusyRegName : Bool <- $$false;
-           Retv.
+  Local Definition resetRule ty : ActionT ty Void
+    := System [
+         DispString _ "[Arbiter.arbiterRule]\n"
+       ];
+       Write busyName : Bool <- $$false;
+       Retv.
 
-    End withTy.
+  Local Definition regs: list RegInitT
+    := makeModule_regs
+         (Register busyName: Bool <- false)%kami.
 
-    Open Scope kami_scope.
-    Open Scope kami_expr_scope.
-
-    Definition regs: list RegInitT
-      := makeModule_regs
-           (Register arbiterBusyRegName: Bool <- false) ++
-           (@FreeList.Ifc.regs freeListParams freelist).
-
-    (* TODO: LLEE: check *)
-    Definition regFiles :=
-      @Build_RegFileBase false 1 arbiterAlistName (Async [arbiterAlistReadName]) arbiterAlistWriteName numTransactions ClientIdTag (@RFNonFile _ _ None) ::
-                         (@FreeList.Ifc.regFiles freeListParams freelist).
-
-    Instance arbiterImpl
-      :  Arbiter
-      := {| Arbiter.Ifc.regs := regs ;
-            Arbiter.Ifc.regFiles := regFiles ;
-            Arbiter.Ifc.sendReq := sendReq ;
-            Arbiter.Ifc.memCallback := memCallback ;
-            Arbiter.Ifc.arbiterRule := arbiterRule |}.
-  End withParams.
-End ArbiterImpl.
+  Definition impl: (Ifc clients)
+    := {| Arbiter.Ifc.regs := regs ;
+          Arbiter.Ifc.regFiles := nil ;
+          Arbiter.Ifc.sendReq := sendReq ;
+          Arbiter.Ifc.callback := callback ;
+          Arbiter.Ifc.resetRule := resetRule |}.
+End Impl.
