Cam/Impl.v
@@ -1,0 +1,87 @@
+Require Import Kami.AllNotations.
+Require Import StdLibKami.RegArray.Ifc.
+Require Import StdLibKami.ReplacementPolicy.Ifc.
+Require Import StdLibKami.Cam.Ifc.
+
+Section Impl.
+  Context {ifcParams: Ifc.Params}.
+
+  Local Open Scope kami_expr.
+  Local Open Scope kami_action.
+
+  Class Params :=
+    {
+      size : nat;
+      policy: @ReplacementPolicy.Ifc.Ifc {|
+                  ReplacementPolicy.Ifc.name := (name ++ ".replacementPolicy")%string;
+                  ReplacementPolicy.Ifc.size := size
+                |};
+  }.
+
+  Context {params: Params}.
+
+  Local Definition Index := Bit (Nat.log2_up size).
+  
+  Local Open Scope kami_scope.
+
+  Local Notation array i := (name ++ ".array_" ++ natToHexStr i)%string.
+  Definition impl: Ifc
+    := {| 
+         regs
+           := map (fun i => (array i,
+                             existT RegInitValT (SyntaxKind (Maybe (Pair keyK dataK)))
+                                    (Some (SyntaxConst (getDefaultConst (Maybe (Pair keyK dataK))))))%string)
+                  (seq 0 size);
+         regFiles
+           := ReplacementPolicy.Ifc.regFiles policy;
+         read
+           := fun ty key ctxt
+                => utila_acts_find_pkt
+                     (map
+                       (fun i : nat
+                         => Read x: Maybe (Pair keyK dataK) <- array i;
+                            LET isMatch <-  #x @% "valid" && matchRead key ctxt (#x @% "data" @% "fst") (#x @% "data" @% "snd");
+                            If #isMatch
+                            then ReplacementPolicy.Ifc.access policy $i;
+                            Ret (STRUCT { "valid" ::= #isMatch ;
+                                          "data" ::= #x @% "data" @% "snd" } : Maybe dataK @# ty))
+                        (seq 0 size));
+
+         write
+           := fun ty key data
+                => GatherActions
+                     (map
+                        (fun i =>
+                           LETA index : Index <- ReplacementPolicy.Ifc.getVictim policy ty;
+                           If ($i == #index)
+                           then Write (array i): Maybe (Pair keyK dataK) <- Valid (STRUCT { "fst" ::= key;
+                                                                                           "snd" ::= data }); Retv;
+                           Retv
+                        )
+                        (seq 0 size)) as _;
+                   Retv;
+
+         flush
+           := fun ty
+                => GatherActions
+                     (map
+                        (fun i =>
+                           Write (array i): Maybe (Pair keyK dataK) <- Invalid;
+                           Retv
+                        )
+                        (seq 0 size)) as _;
+                   Retv;
+         clear
+           := fun ty key ctxt
+                => GatherActions
+                     (map
+                       (fun i : nat
+                          => Read x : Maybe (Pair keyK dataK) <- array i;
+                             If matchClear key ctxt (#x @% "data" @% "fst") (#x @% "data" @% "snd")
+                             then Write (array i) <- $$(getDefaultConst (Maybe (Pair keyK dataK))); Retv;
+                             Retv)
+                        (seq 0 size))
+                     as _;
+                   Retv
+      |}.
+End Impl.
