CompletionBuffer/Impl.v
@@ -1,0 +1,136 @@
+Require Import Kami.AllNotations.
+Require Import StdLibKami.RegArray.Ifc.
+Require Import StdLibKami.FreeList.Ifc.
+Require Import StdLibKami.CompletionBuffer.Ifc.
+
+Section Impl.
+  Context {ifcParams: Ifc.Params}.
+
+  Class Params := { storeArray: @RegArray.Ifc.Ifc {| RegArray.Ifc.name := name ++ ".storeArray";
+                                                     RegArray.Ifc.k := Store;
+                                                     RegArray.Ifc.size := size;
+                                                     RegArray.Ifc.init := None |} ;
+                    resArray: @RegArray.Ifc.Ifc {| RegArray.Ifc.name := name ++ ".resArray";
+                                                   RegArray.Ifc.k := resK;
+                                                   RegArray.Ifc.size := size;
+                                                   RegArray.Ifc.init := None |};
+                    freeList: @FreeList.Ifc.Ifc {| FreeList.Ifc.name := name ++ ".freeList";
+                                                   FreeList.Ifc.size := size |} }.
+
+  Context {params: Params}.
+
+  Local Open Scope kami_expr.
+  Local Open Scope kami_action.
+
+  Local Definition lgSize := Nat.log2_up size.
+  Local Definition Tag := Bit lgSize.
+
+  Local Definition deqPtr := (name ++ ".deqPtr")%string.
+  Local Definition enqPtr := (name ++ ".enqPtr")%string.
+  Local Definition completedArray := (name ++ ".completedArray")%string.
+
+  Local Definition Ptr := Bit (lgSize + 1).
+  
+  Local Definition sendReq
+        (memReq : forall ty, ty OutReq -> ActionT ty (Maybe immResK))
+        ty
+        (req: ty InReq)
+    :  ActionT ty Bool
+    := Read enqPFull: Ptr <- enqPtr;
+       Read deqPFull: Ptr <- deqPtr;
+       Read compds: Array size Bool <- completedArray;
+
+       LET enqP: Tag <- UniBit (TruncLsb _ 1) #enqPFull;
+       LET deqP: Tag <- UniBit (TruncLsb _ 1) #deqPFull;
+       LET outReq
+       :  OutReq
+            <- STRUCT {
+                   "tag"    ::= #enqP;
+                   "outReq" ::= inReqToOutReq (#req @% "inReq") };
+       If (#deqPFull + $(Nat.pow 2 lgSize)) != #enqPFull
+       then
+         If #req @% "sendReq?"
+         then memReq _ outReq
+         else Ret (STRUCT { "valid" ::= $$true;
+                            "data"  ::= $$(getDefaultConst immResK)})
+         as res;
+         If #res @% "valid"
+         then
+           Write enqPtr <- #enqPFull + $1;
+           LET storeVal : Store <- STRUCT { "storeReq" ::= inReqToStoreReq (#req @% "inReq") ;
+                                            "immRes"   ::= #res @% "data" };
+           LET writeRq <- STRUCT { "addr" ::= #enqP;
+                                   "data" ::= #storeVal };
+           LETA _ <- write storeArray _ writeRq;
+           LET isComplete
+             :  Bool
+             <- (IF #req @% "sendReq?"
+                 then isError (#res @% "data")
+                 else $$ true);
+           Write completedArray: Array size Bool <- #compds@[#enqP <- #isComplete];
+           Retv;
+         Ret (#res @% "valid")
+       else Ret $$false
+       as ret;
+       Ret #ret.
+
+  Local Definition callback ty (res: ty InRes): ActionT ty Void :=
+    LET idx: Tag <- #res @% "tag";
+    Read compds: Array size Bool <- completedArray;
+    Write completedArray: Array size Bool <- #compds@[#idx <- $$true];
+    LET writeRq <- STRUCT { "addr" ::= #idx;
+                            "data" ::= #res @% "res" };
+    LETA _ <- write resArray _ writeRq;
+    Retv.
+
+  (* Conceptual rule *)
+  Local Definition callbackRule
+        (callback: forall {ty}, ty OutRes -> ActionT ty Void)
+        ty
+  : ActionT ty Void
+    := Read deqPFull: Ptr <- deqPtr;
+       Read enqPFull: Ptr <- enqPtr;
+       Read compds: Array size Bool <- completedArray;
+       LET deqP: Tag <- UniBit (TruncLsb _ 1) #deqPFull;
+       LETA resVal: resK <- read resArray _ deqP;
+       LETA storeVal: Store <- read storeArray _ deqP;
+       LET res
+       :  OutRes
+          <- STRUCT {
+                 "storeReq" ::= #storeVal @% "storeReq" ;
+                 "immRes"   ::= #storeVal @% "immRes" ;
+                 "res"      ::= #resVal
+               };
+       If (#deqPFull != #enqPFull) && (#compds@[#deqP])
+       then
+         LETA _ <- callback (res : ty OutRes);
+         Write deqPtr <- #deqPFull + $1;
+         Retv;
+       Retv.
+
+  Open Scope kami_scope.
+  Open Scope kami_expr_scope.
+
+  Local Definition regs : list RegInitT
+    := makeModule_regs (
+         Register enqPtr: Ptr <- $ 0 ++
+         Register deqPtr: Ptr <- $ 0 ++
+         Register completedArray: Array size Bool <- Default) ++
+       RegArray.Ifc.regs storeArray ++
+       RegArray.Ifc.regs resArray ++
+       FreeList.Ifc.regs freeList.
+
+  Local Definition regFiles :=
+    RegArray.Ifc.regFiles storeArray ++
+    RegArray.Ifc.regFiles resArray ++
+    FreeList.Ifc.regFiles freeList.
+
+  Definition impl: Ifc :=
+    {|
+      Ifc.regs := regs;
+      Ifc.regFiles := regFiles;
+      Ifc.sendReq := sendReq;
+      Ifc.callbackRule := callbackRule;
+      Ifc.callback := callback;
+    |}.
+End Impl.
