Fetcher/Ifc.v
@@ -1,0 +1,78 @@
+Require Import Kami.AllNotations.
+
+Class Params :=
+  { name : string;
+    size : nat;
+    memReqK : Kind;
+    vAddrSz : nat;
+    compInstSz : nat;
+    immResK : Kind;
+    finalErrK : Kind;
+    isCompressed: forall ty, Bit compInstSz @# ty -> Bool @# ty;
+    isImmErr: forall ty, immResK @# ty -> Bool @# ty;
+    isFinalErr: forall ty, finalErrK @# ty -> Bool @# ty;
+  }.
+
+Section Ifc.
+  Context {params: Params}.
+
+  Definition VAddr    := Bit vAddrSz.
+  Definition ShortVAddr := Bit (vAddrSz - 2).
+  Definition CompInst := Bit compInstSz.
+  Definition InstSz   := compInstSz + compInstSz.
+  Definition Inst     := Bit InstSz.
+
+  Definition TopEntry: Kind
+    := STRUCT_TYPE {
+         "vaddr"  :: ShortVAddr;
+         "immRes" :: immResK;
+         "error"  :: finalErrK;
+         "upper"  :: Maybe CompInst;
+         "lower"  :: Maybe CompInst
+       }.
+  
+  Definition OutReq
+    := STRUCT_TYPE {
+         "inReq" :: STRUCT_TYPE { "memReq" :: memReqK;
+                                  "vaddr"    :: VAddr } ;
+         "sendReq?" :: Bool
+       }.
+
+  Definition InRes
+    := STRUCT_TYPE {
+         "vaddr"  :: VAddr;
+         "immRes" :: immResK;
+         "error"  :: finalErrK;
+         "inst"   :: Inst
+       }.
+
+  (* if inst contains a compressed instruction the upper 16 bit contain arbitrary data. *)
+  Definition OutRes
+    := STRUCT_TYPE {
+         "notComplete?" :: Bool;
+         "vaddr"        :: VAddr;
+         "immRes"       :: immResK;
+         "error"        :: finalErrK;
+         "compressed?"  :: Bool;
+         "errUpper?"    :: Bool;
+         "inst"         :: Inst 
+       }.
+
+  Record Ifc: Type :=
+    {
+      regs: list RegInitT;
+      regFiles : list RegFileBase;
+
+      isFull: forall {ty}, ActionT ty Bool;
+      sendAddr (sendReq: forall ty, ty OutReq -> ActionT ty Bool) ty: ty OutReq -> ActionT ty Bool;
+      callback: forall {ty}, ty InRes -> ActionT ty Void;
+      deq: forall {ty}, ActionT ty Bool;
+      first: forall {ty}, ActionT ty (Maybe OutRes);
+
+      clearTop: forall {ty}, ActionT ty Void;
+      clear: forall {ty}, ActionT ty Void;
+
+      notCompleteDeqRule: forall {ty}, ActionT ty Void;
+      transferRule: forall {ty}, ActionT ty Void;
+    }.
+End Ifc.
