Fifo/Impl.v
@@ -1,0 +1,88 @@
+Require Import Kami.AllNotations.
+Require Import StdLibKami.RegArray.Ifc.
+Require Import StdLibKami.Fifo.Ifc.
+
+Section Impl.
+  Context {ifcParams : Ifc.Params}.
+
+  Class Params := { sizePow2: Nat.pow 2 (Nat.log2_up size) = size ;
+                    regArray  : @RegArray.Ifc.Ifc {| RegArray.Ifc.name := name ++ ".regArray" ;
+                                                     RegArray.Ifc.k := k ;
+                                                     RegArray.Ifc.size := size;
+                                                     RegArray.Ifc.init := None |} }.
+
+  Context {params: Params}.
+
+  Local Definition twoSize := 2 * size.
+
+  Local Definition deqPtrName := (name ++ ".deqPtr")%string.
+  Local Definition enqPtrName := (name ++ ".enqPtr")%string.
+  
+  Local Open Scope kami_expr.
+  Local Open Scope kami_action.
+
+  Local Definition fastModSize ty (w : Bit (lgSize + 1) @# ty): Bit lgSize @# ty :=
+    UniBit (TruncLsb lgSize 1) w.
+
+  Local Definition isEmpty ty: ActionT ty Bool :=
+    Read deq: Bit (lgSize + 1) <- deqPtrName;
+    Read enq: Bit (lgSize + 1) <- enqPtrName;
+    Ret (#deq == #enq).
+
+  Local Definition isFull ty: ActionT ty Bool :=
+    Read deq: Bit (lgSize + 1) <- deqPtrName;
+    Read enq: Bit (lgSize + 1) <- enqPtrName;
+    Ret ((#deq + $size) == #enq).
+  
+  Local Definition numFree ty: ActionT ty (Bit lgSize) :=
+    Read deq: Bit (lgSize + 1) <- deqPtrName;
+    Read enq: Bit (lgSize + 1) <- enqPtrName;
+    Ret (UniBit (TruncLsb _ 1) ($size - (#enq - #deq))).
+  
+  Local Definition first ty: ActionT ty (Maybe k) := 
+    LETA empty: Bool <- isEmpty ty;
+    Read deq: Bit (lgSize + 1) <- deqPtrName;
+    LET idx: Bit lgSize <- (fastModSize #deq);
+    LETA dat: k <- read regArray ty idx;
+    Ret (STRUCT { "valid" ::= !#empty; "data" ::= #dat} : Maybe k @# ty).
+
+  Local Definition deq ty: ActionT ty (Maybe k) :=
+    LETA data: Maybe k <- first ty;
+    Read deq: Bit (lgSize + 1) <- deqPtrName;
+    Write deqPtrName: Bit (lgSize + 1) <- #deq + (IF #data @% "valid" then $1 else $0);
+    Ret #data.
+
+  Local Definition enq ty (new: ty k): ActionT ty Bool :=
+    Read enq: Bit (lgSize + 1) <- enqPtrName;
+    LET idx: Bit lgSize <- (fastModSize #enq);
+    LETA full: Bool <- isFull ty;
+    If !#full then (
+      LET writeRq <- STRUCT { "addr" ::= #idx; "data" ::= #new };
+      LETA _ <- write regArray _ writeRq;
+      Write enqPtrName: Bit (lgSize + 1) <- #enq + $1;
+      Retv
+      );
+    Ret !#full.
+    
+  Local Definition flush ty: ActionT ty Void :=
+    Write deqPtrName: Bit (lgSize + 1) <- $0;
+    Write enqPtrName: Bit (lgSize + 1) <- $0;
+    Retv.
+
+  Local Definition regs: list RegInitT := makeModule_regs ( Register deqPtrName: Bit (lgSize + 1) <- Default ++
+                                                            Register enqPtrName: Bit (lgSize + 1) <- Default )%kami
+                                                          ++ RegArray.Ifc.regs regArray.
+
+  Definition impl: Ifc :=
+    {|
+      Ifc.regs := regs;
+      Ifc.regFiles := RegArray.Ifc.regFiles regArray;
+      Ifc.isEmpty := isEmpty;
+      Ifc.isFull := isFull;
+      Ifc.numFree := numFree;
+      Ifc.first := first;
+      Ifc.deq := deq;
+      Ifc.enq := enq;
+      Ifc.flush := flush
+    |}.
+End Impl.
