FreeList/Array.v
@@ -1,66 +1,58 @@
-(*
-  Represents a free list that uses a boolean array register rather
-  than a Fifo.
-*)
 Require Import Kami.AllNotations.
 Require Import Kami.Utila.
 Require Import StdLibKami.FreeList.Ifc.
 
-Section array.
-  Context {freeListParams : FreeListParams}.
+Section Impl.
+  Context {ifcParams : Ifc.Params}.
 
   Local Definition arrayRegName := (name ++ ".data")%string.
 
-  Section arrayParams.
-    Local Definition len := Nat.pow 2 tagSz.
-    Local Definition Tag := Bit tagSz.
+  Local Definition Tag := Bit lgSize.
 
-    Local Open Scope kami_expr.
-    Local Open Scope kami_action.
+  Local Open Scope kami_expr.
+  Local Open Scope kami_action.
 
-    Local Definition initialize ty: ActionT ty Void :=
-      Write arrayRegName: Array len Bool <- BuildArray (fun _ => $$false);
-      Retv.
+  Local Definition initialize ty: ActionT ty Void :=
+    Write arrayRegName: Array size Bool <- BuildArray (fun _ => $$false);
+    Retv.
 
-    Local Definition nextToAlloc ty: ActionT ty (Maybe Tag) := 
-      Read freeArray: Array len Bool <- arrayRegName;
-      Ret (fold_left
-             (fun (tag : Maybe Tag @# ty) (index : nat)
-              => (IF tag @% "valid"
-                  then tag
-                  else STRUCT {
-                           "valid" ::= !(#freeArray@[$index : Tag @# ty]);
-                           "data" ::= ($index : Tag @# ty)
-                         }))
-                   (seq 0 len)
-             Invalid).
-  
-    Local Definition alloc ty (tag: ty Tag): ActionT ty Bool := 
-      Read freeArray: Array len Bool <- arrayRegName;
-      LET res: Bool <- #freeArray@[#tag];
-      Write arrayRegName: Array len Bool <- #freeArray@[#tag <- $$true];
-      Ret !#res.
-  
-    Local Definition free ty (tag: ty Tag): ActionT ty Void :=
-      Read freeArray: Array len Bool <- arrayRegName;                                                        
-      Write arrayRegName: Array len Bool <- #freeArray@[#tag <- $$false];
-      Retv.
+  Local Definition nextToAlloc ty: ActionT ty (Maybe Tag) := 
+    Read freeArray: Array size Bool <- arrayRegName;
+    Ret (fold_left
+           (fun (tag : Maybe Tag @# ty) (index : nat)
+            => (IF tag @% "valid"
+                then tag
+                else STRUCT {
+                         "valid" ::= !(#freeArray@[$index : Tag @# ty]);
+                         "data" ::= ($index : Tag @# ty)
+                       }))
+                 (seq 0 size)
+           Invalid).
 
-    Local Definition regs: list RegInitT := makeModule_regs ( Register arrayRegName: Array len Bool <- Default )%kami.
+  Local Definition alloc ty (tag: ty Tag): ActionT ty Bool := 
+    Read freeArray: Array size Bool <- arrayRegName;
+    LET res: Bool <- #freeArray@[#tag];
+    Write arrayRegName: Array size Bool <- #freeArray@[#tag <- $$true];
+    Ret !#res.
 
-    Definition arrayFreeList: FreeList :=
-      {|
-        FreeList.Ifc.regs := regs;
-        FreeList.Ifc.regFiles := nil;
-        FreeList.Ifc.length := len;
-        FreeList.Ifc.initialize := initialize;
-        FreeList.Ifc.nextToAlloc := nextToAlloc;
-        FreeList.Ifc.alloc := alloc;
-        FreeList.Ifc.free := free
-      |}.
+  Local Definition free ty (tag: ty Tag): ActionT ty Void :=
+    Read freeArray: Array size Bool <- arrayRegName;                                                        
+    Write arrayRegName: Array size Bool <- #freeArray@[#tag <- $$false];
+    Retv.
 
-    Local Close Scope kami_action.
-    Local Close Scope kami_expr.
+  Local Definition regs: list RegInitT := makeModule_regs ( Register arrayRegName: Array size Bool <- Default )%kami.
 
-  End arrayParams.
-End array.
+  Definition impl: Ifc :=
+    {|
+      Ifc.regs := regs;
+      Ifc.regFiles := nil;
+      Ifc.initialize := initialize;
+      Ifc.nextToAlloc := nextToAlloc;
+      Ifc.alloc := alloc;
+      Ifc.free := free
+    |}.
+
+  Local Close Scope kami_action.
+  Local Close Scope kami_expr.
+
+End Impl.
