FreeList/Proofs.v
@@ -112,74 +112,74 @@
 
 
 
-Require Import Kami.All.
-Require Import StdLibKami.FreeList.Spec.
-Require Import StdLibKami.FreeList.Ifc.
-Require Import StdLibKami.FreeList.Array.
-Require Import Coq.Logic.EqdepFacts.
-Require Import Kami.GallinaModules.Relations.
-Require Import Kami.GallinaModules.AuxTactics.
-Require Import Kami.GallinaModules.AuxLemmas.
+(* Require Import Kami.All. *)
+(* Require Import StdLibKami.FreeList.Spec. *)
+(* Require Import StdLibKami.FreeList.Ifc. *)
+(* Require Import StdLibKami.FreeList.Array. *)
+(* Require Import Coq.Logic.EqdepFacts. *)
+(* Require Import Kami.GallinaModules.Relations. *)
+(* Require Import Kami.GallinaModules.AuxTactics. *)
+(* Require Import Kami.GallinaModules.AuxLemmas. *)
 
-Record FreeListCorrect {FLParams} (imp spec: @FreeList FLParams): Type :=
-  {
-    freeListRegs: list (Attribute FullKind);
-    freeListR: RegsT -> RegsT -> Prop;
-    nextToAllocCorrect: EffectlessRelation freeListR (@nextToAlloc _ imp type) (@nextToAlloc _ spec type);
-    nextToAllocWb: ActionWb freeListRegs (@nextToAlloc _ imp type);
-    allocCorrect: forall allocand, EffectfulRelation freeListR (@alloc _ imp type allocand) (@alloc _ spec type allocand);
-    allocWb: forall allocand, ActionWb freeListRegs (@alloc _ imp type allocand);
-    freeCorrect: forall input, EffectfulRelation freeListR (@free _ imp type input) (@free _ spec type input);
-    freeWb: forall input, ActionWb freeListRegs (@free _ imp type input);
-  }.
+(* Record FreeListCorrect {FLParams} (imp spec: @FreeList FLParams): Type := *)
+(*   { *)
+(*     freeListRegs: list (Attribute FullKind); *)
+(*     freeListR: RegsT -> RegsT -> Prop; *)
+(*     nextToAllocCorrect: EffectlessRelation freeListR (@nextToAlloc _ imp type) (@nextToAlloc _ spec type); *)
+(*     nextToAllocWb: ActionWb freeListRegs (@nextToAlloc _ imp type); *)
+(*     allocCorrect: forall allocand, EffectfulRelation freeListR (@alloc _ imp type allocand) (@alloc _ spec type allocand); *)
+(*     allocWb: forall allocand, ActionWb freeListRegs (@alloc _ imp type allocand); *)
+(*     freeCorrect: forall input, EffectfulRelation freeListR (@free _ imp type input) (@free _ spec type input); *)
+(*     freeWb: forall input, ActionWb freeListRegs (@free _ imp type input); *)
+(*   }. *)
 
-Section Proofs.
-  Context `{Params : FreeListParams}.
+(* Section Proofs. *)
+(*   Context `{Params : FreeListParams}. *)
 
-  Definition spFreeList := @specFreeList Params.
-  Definition arrFreeList := @arrayFreeList Params.
+(*   Definition spFreeList := @specFreeList Params. *)
+(*   Definition arrFreeList := @arrayFreeList Params. *)
     
-  Record myArrayFreeListR (o_i o_s : RegsT) : Prop :=
-    {
-      LocalReg : RegT;
-      ArrayVal : Fin.t Array.len -> bool;
-      LocalRegVal : LocalReg = (Array.arrayRegName, existT _ (SyntaxKind (Array Array.len Bool)) ArrayVal);
-      Ho_iCorrect : o_i = [LocalReg];
-      Ho_sCorrect : o_s = [LocalReg];
-      Ho_iNoDup : NoDup (map fst o_i);
-      Ho_sNoDup : NoDup (map fst o_s)
-    }.
+(*   Record myArrayFreeListR (o_i o_s : RegsT) : Prop := *)
+(*     { *)
+(*       LocalReg : RegT; *)
+(*       ArrayVal : Fin.t Array.len -> bool; *)
+(*       LocalRegVal : LocalReg = (Array.arrayRegName, existT _ (SyntaxKind (Array Array.len Bool)) ArrayVal); *)
+(*       Ho_iCorrect : o_i = [LocalReg]; *)
+(*       Ho_sCorrect : o_s = [LocalReg]; *)
+(*       Ho_iNoDup : NoDup (map fst o_i); *)
+(*       Ho_sNoDup : NoDup (map fst o_s) *)
+(*     }. *)
   
-  Ltac Record_destruct :=
-    match goal with
-    | [ H : myArrayFreeListR _ _ |- _] => destruct H
-    end.
+(*   Ltac Record_destruct := *)
+(*     match goal with *)
+(*     | [ H : myArrayFreeListR _ _ |- _] => destruct H *)
+(*     end. *)
   
   
 
-  (* Goal FreeListCorrect arrFreeList spFreeList. *)
-  (*   econstructor 1 with (freeListR := myArrayFreeListR) *)
-  (*                       (freeListRegs := [(Array.arrayRegName, SyntaxKind (Array Array.len Bool))]). *)
-  (*   all : *)
-  (*     intros *)
-  (*     ; unfold EffectfulRelation, EffectlessRelation, ActionWb *)
-  (*     ; intros *)
-  (*     ; try Record_destruct *)
-  (*     ; try (destruct LocalReg; inv LocalRegVal) *)
-  (*     ; unfold nextToAlloc, alloc, free, arrayFreeList, specFreeList, arrFreeList, spFreeList, *)
-  (*       arrayFreeList, specFreeList, Array.nextToAlloc, Spec.nextToAlloc in *. *)
-  (*   - hyp_consumer1. *)
-  (*     + goal_consumer. *)
-  (*       my_simpl_solver. *)
-  (*       goal_consumer. *)
-  (*       my_simpl_solver. *)
-  (*       repeat goal_consumer. *)
-  (*       3 : { reflexivity. *)
-  (*       } *)
-  (*       3 : auto. *)
-  (*       3 : auto. *)
-  (*       3 : auto. *)
-  (*       unfold Array.arrayRegName. *)
-  (*       unfold Spec.arrayRegName. *)
-  (*       auto. *)
-End Proofs.
+(*   (* Goal FreeListCorrect arrFreeList spFreeList. *) *)
+(*   (*   econstructor 1 with (freeListR := myArrayFreeListR) *) *)
+(*   (*                       (freeListRegs := [(Array.arrayRegName, SyntaxKind (Array Array.len Bool))]). *) *)
+(*   (*   all : *) *)
+(*   (*     intros *) *)
+(*   (*     ; unfold EffectfulRelation, EffectlessRelation, ActionWb *) *)
+(*   (*     ; intros *) *)
+(*   (*     ; try Record_destruct *) *)
+(*   (*     ; try (destruct LocalReg; inv LocalRegVal) *) *)
+(*   (*     ; unfold nextToAlloc, alloc, free, arrayFreeList, specFreeList, arrFreeList, spFreeList, *) *)
+(*   (*       arrayFreeList, specFreeList, Array.nextToAlloc, Spec.nextToAlloc in *. *) *)
+(*   (*   - hyp_consumer1. *) *)
+(*   (*     + goal_consumer. *) *)
+(*   (*       my_simpl_solver. *) *)
+(*   (*       goal_consumer. *) *)
+(*   (*       my_simpl_solver. *) *)
+(*   (*       repeat goal_consumer. *) *)
+(*   (*       3 : { reflexivity. *) *)
+(*   (*       } *) *)
+(*   (*       3 : auto. *) *)
+(*   (*       3 : auto. *) *)
+(*   (*       3 : auto. *) *)
+(*   (*       unfold Array.arrayRegName. *) *)
+(*   (*       unfold Spec.arrayRegName. *) *)
+(*   (*       auto. *) *)
+(* End Proofs. *)
