Router/Impl.v
@@ -1,0 +1,72 @@
+Require Import Kami.AllNotations.
+Require Import StdLibKami.Router.Ifc.
+
+Section Impl.
+  Context {params: Params}.
+  
+  Local Definition routedReg := (Router.Ifc.name ++ ".routedReg")%string.
+  
+  Local Open Scope kami_expr_scope.
+  Local Open Scope kami_action_scope.
+  
+  Section withTy.
+    Context (ty: Kind -> Type).
+    
+    Local Definition pollRuleGenerator (clientCallback: forall {ty}, ty respK -> ActionT ty Void) (dev: Fin.t numDevices): ActionT ty Void :=
+      System [
+        DispString _ "[Router.pollRuleGenerator]\n"
+      ];
+      Read alreadyRoutedReg: Bool <- routedReg;
+      If !#alreadyRoutedReg then (
+        LETA resp: Maybe respK <- (nth_Fin devices dev).(devicePoll);
+        LET respDat: respK <- (#resp @% "data");
+        If (#resp @% "valid") then (
+            System [
+              DispString _ ("[Router.pollRuleGenerator] forwarding response from device: " ++ natToHexStr (proj1_sig (Fin.to_nat dev)) ++ "\n")
+            ];
+            LETA _ <- clientCallback respDat;
+            Write routedReg: Bool <- $$true;
+            Retv
+        );
+        Retv
+      );
+      Retv.
+
+    Local Definition pollingDone: ActionT ty Void :=
+      System [
+        DispString _ "[Router.pollingDone]\n"
+      ];
+      Write routedReg: Bool <- $$false;
+      Retv.
+
+    Local Definition sendReq (req: ty OutReq) : ActionT ty Bool :=
+      System [
+        DispString _ "[Router.req]\n"
+      ];
+      GatherActions (map (fun i =>
+                            LET req_real: reqK <- #req @% "req";
+                            If ($(proj1_sig (Fin.to_nat i)) == #req @% "dtag")
+                            then
+                              System [
+                                DispString _ "[Router.req] sending request to device: ";
+                                DispHex (#req @% "dtag");
+                                DispString _ "\n"
+                              ];
+                              (nth_Fin devices i).(deviceReq) req_real
+                            else Ret $$false as ret;
+                            Ret #ret
+                         ) (getFins numDevices)) as accepted; Ret (@Kor _ Bool accepted).
+  End withTy.
+  
+  Local Definition pollRules (clientCallback: forall ty, ty respK -> ActionT ty Void) :=
+    (map (fun dev ty => pollRuleGenerator ty clientCallback dev) (getFins numDevices)) ++ [pollingDone].
+
+  Local Definition regs: list RegInitT := makeModule_regs ( Register routedReg: Bool <- false )%kami.
+  
+  Definition impl: Ifc
+    := {| Ifc.regs := regs ;
+          Ifc.regFiles := nil ;
+          Ifc.sendReq := sendReq;
+          Ifc.pollRules := pollRules |}.
+
+End Impl.
